fixed equality & syntax auxlilary defs

deps/poulet4/lib/P4cub/Syntax/Equality.v
@@ -1,649 +1,305 @@
-Set Warnings "-custom-entry-overridden".
 Require Import Coq.PArith.BinPosDef Coq.PArith.BinPos
         Coq.ZArith.BinIntDef Coq.ZArith.BinInt
         Coq.NArith.BinNatDef Coq.NArith.BinNat
         Poulet4.P4cub.Syntax.AST Poulet4.P4cub.Syntax.IndPrincip
         Poulet4.P4cub.Syntax.CubNotations.
+Import Expr ExprNotations.
 
-Reserved Notation "∮ e1 ≡ e2"
-         (at level 200, e1 custom p4expr, e2 custom p4expr, no associativity).
+Reserved Infix "=?" (at level 70).
 
-Module TypeEquivalence.
-  Import Field.FieldTactics Expr TypeNotations.
+Fixpoint eqbt (τ1 τ2 : t) {struct τ1} : bool :=
+  let fix eqbl (ts1 ts2 : list t) {struct ts1} : bool :=
+    match ts1, ts2 with
+    | [], []           => true
+    | t1::ts1', t2::ts2' => ((t1 =? t2)%ty && eqbl ts1' ts2')%bool
+    | _, _             => false
+    end in
+  match τ1, τ2 with
+  | TBool, TBool
+  | TError, TError                 => true
+  | TVar X1, TVar X2               => Nat.eqb X1 X2
+  | TBit w1, TBit w2               => (w1 =? w2)%N
+  | TInt w1, TInt w2               => (w1 =? w2)%positive
+  | TStruct ts1 b1, TStruct ts2 b2 => (eqb b1 b2) && eqbl ts1 ts2
+  | _, _ => false
+  end
+where "x '=?' y" := (eqbt x y) : ty_scope.
+
+Section TypeEquivalence.
+  Hint Rewrite PeanoNat.Nat.eqb_refl : core.
+  Hint Rewrite Pos.eqb_refl : core.
+  Hint Rewrite @eqb_list_refl : core.
+  Hint Rewrite @equiv_dec_refl : core.
+  Hint Rewrite N.eqb_refl.
+  Hint Extern 4 => equiv_dec_refl_tactic : core.
+  Hint Rewrite eqb_reflx : core.
   
-  Section TypeEquivalence.
-    (** Decidable equality. *)
-    Fixpoint eqbt (τ1 τ2 : t) : bool :=
-      let fix lstruct (ts1 ts2 : list t) : bool :=
-          match ts1, ts2 with
-          | [], [] => true
-          | t1::ts1, t2::ts2 => eqbt t1 t2 && lstruct ts1 ts2
-          | [], _::_ | _::_, [] => false
-          end in
-      let fix fstruct (ts1 ts2 : F.fs String.string t) : bool :=
-          match ts1, ts2 with
-          | [], [] => true
-          | (x1,t1)::ts1, (x2,t2)::ts2
-            => equiv_dec x1 x2 &&&& eqbt t1 t2 && fstruct ts1 ts2
-          | [], _::_ | _::_, [] => false
-          end in
-      match τ1, τ2 with
-      | TVar X1, TVar X2 => String.eqb X1 X2
-      | {{ Bool }}, {{ Bool }}
-      | {{ error }}, {{ error }} => true
-      | {{ bit<w1> }}, {{ bit<w2> }} => (w1 =? w2)%N
-      | {{ int<w1> }}, {{ int<w2> }} => (w1 =? w2)%positive
-      | {{ tuple ts1 }}, {{ tuple ts2 }} => lstruct ts1 ts2
-      | {{ hdr { ts1 } }}, {{ hdr { ts2 } }}
-      | {{ struct { ts1 } }}, {{ struct { ts2 } }} => fstruct ts1 ts2
-      | {{ stack ts1[n1] }}, {{ stack ts2[n2] }}
-        => (n1 =? n2)%positive && fstruct ts1 ts2
-      | _, _ => false
-      end.
-    (**[]*)
-
-    Hint Rewrite String.eqb_refl : core.
-    Hint Rewrite Pos.eqb_refl : core.
-    Hint Rewrite @eqb_list_refl : core.
-    Hint Rewrite @equiv_dec_refl : core.
-    Hint Extern 4 => equiv_dec_refl_tactic : core.
+  Lemma eqbt_refl : forall τ, (τ =? τ)%ty = true.
+  Proof.
+    induction τ using custom_t_ind; unravel;
+      autorewrite with core; auto;
+      try ind_list_Forall;
+      intuition; autorewrite with core;
+      repeat (rewrite_true; unravel); auto.
+  Qed.
     
-    Lemma eqbt_refl : forall τ, eqbt τ τ = true.
-    Proof.
-      Hint Rewrite Pos.eqb_refl.
-      Hint Rewrite N.eqb_refl.
-      Hint Rewrite equiv_dec_refl.
-      Hint Extern 0 => equiv_dec_refl_tactic : core.
-      induction τ using custom_t_ind; unravel;
-        autorewrite with core; auto;
-          try ind_list_Forall; try ind_list_predfs;
-            intuition; autorewrite with core;
-              repeat (rewrite_true; unravel); auto.
-    Qed.
-    
-    Ltac eauto_too_dumb :=
-      match goal with
-      | H: ?f ?x ?y = ?z,
-           IH: (forall y, ?f ?x y = ?z -> _)
-        |- _ => apply IH in H; clear IH
-      end.
+  Ltac eauto_too_dumb :=
+    match goal with
+    | H: ?f ?x ?y = ?z,
+        IH: (forall y, ?f ?x y = ?z -> _)
+      |- _ => apply IH in H; clear IH
+    end.
 
-    Ltac helper :=
-      match goal with
-      | H: String.eqb _ _ = true
-        |- _ => rewrite String.eqb_eq in H; subst; auto
-      | H: (_ =? _)%positive = true
-        |- _ => apply Peqb_true_eq in H; subst; auto
-      | H: eqb_list _ _ = true
-        |- _ => apply eqb_list_eq in H
-      end.
-
-    Hint Extern 5 => helper : core.
+  Local Hint Resolve eqb_prop : core.
+  Local Hint Resolve PeanoNat.Nat.eqb_eq : core.
+  Local Hint Resolve Peqb_true_eq : core.
     
-    Lemma eqbt_eq : forall t1 t2, eqbt t1 t2 = true -> t1 = t2.
-    Proof.
-      induction t1 using custom_t_ind; intros []; intros; unravel in *;
-        try discriminate; repeat destruct_andb; auto; f_equal;
-          repeat destruct_lifted_andb; unravel in *; subst; auto;
-          try match goal with
-              | IH: Forall _ ?ts1,
-                    H: _ ?ts1 ?ts2 = true
-                |- _ => generalize dependent ts2;
-                        induction ts1; intros []; intros;
-                          try discriminate; try inv_Forall_cons;
-                            repeat destruct_andb; intuition;
-                              repeat eauto_too_dumb; subst; auto
-              end;
-          try match goal with
-              | IH: F.predfs_data _ ?ts1,
-                    H: _ ?ts1 ?ts2 = true
-                |- _ => generalize dependent ts2;
-                        induction ts1; intros [| [? ?] ?]; intros;
-                          try discriminate; try invert_cons_predfs;
-                            try destruct_lifted_andb;
-                            repeat destruct_andb; intuition;
-                              unfold equiv in *; subst;
-                                repeat eauto_too_dumb; subst; auto
-              end.
+  Ltac helper :=
+    match goal with
+    | H: Nat.eqb _ _ = true
+      |- _ => apply PeanoNat.Nat.eqb_eq in H; subst; auto
+    | H: String.eqb _ _ = true
+      |- _ => rewrite String.eqb_eq in H; subst; auto
+    | H: (_ =? _)%positive = true
+      |- _ => apply Peqb_true_eq in H; subst; auto
+    | H: eqb_list _ _ = true
+      |- _ => apply eqb_list_eq in H
+    end.
+
+  Hint Extern 5 => helper : core.
+    
+  Lemma eqbt_eq : forall t1 t2, (t1 =? t2)%ty = true -> t1 = t2.
+  Proof.
+    induction t1 using custom_t_ind; intros []; intros; unravel in *;
+      try discriminate; repeat destruct_andb; auto; f_equal;
+      repeat destruct_lifted_andb; unravel in *; subst; auto;
+      try match goal with
+          | IH: Forall _ ?ts1,
+              H: _ ?ts1 ?ts2 = true
+            |- _ => generalize dependent ts2;
+                  induction ts1; intros []; intros;
+                  try discriminate; try inv_Forall_cons;
+                  repeat destruct_andb; intuition;
+                  repeat eauto_too_dumb; subst; auto
+          end;
       auto using InitialRing.Neqb_ok.
-    Qed.
+  Qed.
     
-    Lemma eqbt_eq_iff : forall t1 t2 : t,
-        eqbt t1 t2 = true <-> t1 = t2.
-    Proof.
-      Hint Resolve eqbt_refl : core.
-      Hint Resolve eqbt_eq : core.
-      intros t1 t2; split; intros; subst; auto.
-    Qed.
+  Lemma eqbt_eq_iff : forall t1 t2 : t,
+      (t1 =? t2)%ty = true <-> t1 = t2.
+  Proof.
+    Hint Resolve eqbt_refl : core.
+    Hint Resolve eqbt_eq : core.
+    intros t1 t2; split; intros; subst; auto.
+  Qed.
     
-    Lemma eqbt_reflect : forall t1 t2, reflect (t1 = t2) (eqbt t1 t2).
-    Proof.
-      Hint Resolve eqbt_eq_iff : core.
-      intros; reflect_split; auto.
-      apply eqbt_eq_iff in H;
-        rewrite H in Heqb; discriminate.
-    Defined.
+  Lemma eqbt_reflect : forall t1 t2, reflect (t1 = t2) (t1 =? t2)%ty.
+  Proof.
+    Hint Resolve eqbt_eq_iff : core.
+    intros; reflect_split; auto.
+    apply eqbt_eq_iff in H;
+      rewrite H in Heqb; discriminate.
+  Defined.
     
-    Transparent eqbt_reflect.
+  Transparent eqbt_reflect.
 
-    Lemma eq_dec : forall t1 t2 : t,
-        t1 = t2 \/ t1 <> t2.
-    Proof.
-      intros t1 t2. pose proof eqbt_reflect t1 t2 as H.
-      inv H; auto.
-    Qed.
-  End TypeEquivalence.
-  
-  Global Instance TypeEqDec : EqDec t eq :=
-    { equiv_dec := fun t1 t2 => reflect_dec _ _ (eqbt_reflect t1 t2) }.
-  (**[]*)
+  Lemma eq_dec : forall t1 t2 : t,
+      t1 = t2 \/ t1 <> t2.
+  Proof.
+    intros t1 t2. pose proof eqbt_reflect t1 t2 as H.
+    inv H; auto.
+  Qed.
 End TypeEquivalence.
+  
+Global Instance TypeEqDec : EqDec t eq :=
+  { equiv_dec := fun t1 t2 => reflect_dec _ _ (eqbt_reflect t1 t2) }.
+(**[]*)
+End TypeEquivalence.
+  
+Instance TypeEqDec : EqDec t eq :=
+  { equiv_dec := fun t1 t2 => reflect_dec _ _ (eqbt_reflect t1 t2) }.
 
 (** Decidable Expression Equivalence. *)
-Module ExprEquivalence.
-  Import Field.FieldTactics Expr
-         TypeNotations UopNotations BopNotations
-         MatchkindNotations ExprNotations TypeEquivalence.
+Global Instance UopEqDec : EqDec uop eq.
+Proof.
+  intros [] []; unravel in *;
+    try match goal with
+        | n1 : positive, n2: positive
+          |- _ => destruct (Pos.eq_dec n1 n2) as [? | ?]; subst; auto
+        end; auto 2;
+    try (right; intros ?; try discriminate;
+         inv_eq; try contradiction).
+Defined.
   
-  Global Instance UopEqDec : EqDec uop eq.
-  Proof.
-    intros [] []; unravel in *;
-      try match goal with
-          | n1 : positive, n2: positive
-            |- _ => destruct (Pos.eq_dec n1 n2) as [? | ?]; subst; auto
-          end; auto 2;
-        try (right; intros ?; try discriminate;
-             inv_eq; try contradiction).
-  Defined.
-  
-  Global Instance BopEqDec : EqDec bop eq.
-  Proof.
-    intros [] []; unfold equiv, complement in *;
-      auto 2; right; intros ?; discriminate.
-  Defined.
+Global Instance BopEqDec : EqDec bop eq.
+Proof.
+  intros [] []; unfold equiv, complement in *;
+    auto 2; right; intros ?; discriminate.
+Defined.
+    
+(** Decidable Expression Equivalence. *)
+Fixpoint eqbe (e1 e2 : e) : bool :=
+  let fix lstruct (es1 es2 : list e) : bool :=
+    match es1, es2 with
+    | [], _::_ | _::_, [] => false
+    | [], [] => true
+    | e1::es1, e2::es2 => (e1 =? e2)%expr && lstruct es1 es2
+    end in
+  let opb (o1 o2 : option e) : bool :=
+    match o1, o2 with
+    | Some e1, Some e2 => (e1 =? e2)%expr
+    | None,    None    => true
+    | _, _             => false
+    end in
+  match e1, e2 with
+  | EBool b1, EBool b2 => eqb b1 b2
+  | w1 `W n1, w2 `W n2
+    => (w1 =? w2)%N && (n1 =? n2)%Z
+  | w1 `S z1, w2 `S z2
+    => (w1 =? w2)%positive && (z1 =? z2)%Z
+  | EVar τ1 x1, EVar τ2 x2
+    => PeanoNat.Nat.eqb x1 x2 && (τ1 =? τ2)%ty
+  | ESlice e1 h1 l1, ESlice e2 h2 l2
+    => (h1 =? h2)%positive && (l1 =? l2)%positive && (e1 =? e2)%expr
+  | ECast τ1 e1, ECast τ2 e2
+    => (τ1 =? τ2)%ty && (e1 =? e2)%expr
+  | EUop t2 u1 e1, EUop t1 u2 e2
+    => equiv_dec u1 u2 &&&& (e1 =? e2)%expr && (t1 =? t2)%ty
+  | EBop t1 o1 el1 er1, EBop t2 o2 el2 er2
+    => equiv_dec o1 o2 &&&& (el1 =? el2)%expr && (er1 =? er2)%expr && (t1 =? t2)%ty
+  | EStruct fs1 e1, EStruct fs2 e2
+    => opb e1 e2 && lstruct fs1 fs2
+  | EMember t1 x1 e1, EMember t2 x2 e2
+    => PeanoNat.Nat.eqb x1 x2 && (e1 =? e2)%expr && (t1 =? t2)%ty
+  | EError err1, EError err2
+    => if equiv_dec err1 err2 then true else false
+  | _, _ => false
+  end
+where "x '=?' y" := (eqbe x y) : expr_scope.
 
-  Global Instance MatchKindEqDec : EqDec Expr.matchkind eq.
+Section ExprEquivalenceDefs.
+  Hint Rewrite eqb_reflx : core.
+  Hint Rewrite Pos.eqb_refl : core.
+  Hint Rewrite Z.eqb_refl : core.
+  Hint Rewrite eqbt_refl : core.
+  Local Hint Extern 5 => equiv_dec_refl_tactic : core.
+  Hint Rewrite PeanoNat.Nat.eqb_refl : core.
+  Hint Rewrite @eqb_list_refl : core.
+  Hint Rewrite @equiv_dec_refl : core.
+  Hint Rewrite N.eqb_refl : core.
+  Hint Rewrite eqb_reflx : core.
+
+  Lemma eqbe_refl : forall exp : e, (exp =? exp)%expr = true.
+>>>>>>> 9252317b9 (fixed equality & syntax auxlilary defs)
   Proof.
-    unfold EqDec; unfold equiv, complement.
-    intros [] []; try (left; reflexivity);
-      try (right; intros H; inversion H).
-  Defined.
+    intro exp; induction exp using custom_e_ind;
+      cbn; autorewrite with core;
+      try match goal with
+          | H: predop _ _ |- _ => inv H
+          end;
+      try ind_list_Forall; cbn in *;
+      repeat match goal with
+             | H: ?trm = true |- context [ ?trm ] => rewrite H; clear H
+             end; cbn in *; auto.
+    intuition; apply andb_prop in H as [H1 H2]; auto.
+  Qed.
+
+  Local Hint Resolve eqb_prop : core.
+  Local Hint Resolve PeanoNat.Nat.eqb_eq : core.
+  Local Hint Resolve EqNat.beq_nat_true : core.
+  Local Hint Resolve Peqb_true_eq : core.
   
-  (** Equality of expressions. *)
-  Inductive equive {tags_t : Type} : e tags_t -> e tags_t -> Prop :=
-  | equive_bool b i i' :
-      ∮ BOOL b @ i ≡ BOOL b @ i'
-  | equive_bit w n i i' :
-      ∮ w W n @ i ≡ w W n @ i'
-  | equive_int w z i i' :
-      ∮ w S z @ i ≡ w S z @ i'
-  | equive_var x τ i1 i2 :
-      ∮ Var x:τ @ i1 ≡ Var x:τ @ i2
-  | equive_slice e1 e2 h l i1 i2 :
-      ∮ e1 ≡ e2 ->
-      ∮ Slice e1 [h:l] @ i1 ≡ Slice e2 [h:l] @ i2
-  | equive_cast τ e1 e2 i1 i2 :
-      ∮ e1 ≡ e2 ->
-      ∮ Cast e1:τ @ i1 ≡ Cast e2:τ @ i2
-  | equive_uop t op e1 e2 i1 i2 :
-      ∮ e1 ≡ e2 ->
-      ∮ UOP op e1 : t @ i1 ≡ UOP op e2 : t @ i2
-  | equive_bop t op el1 er1 el2 er2 i1 i2 :
-      ∮ el1 ≡ el2 ->
-      ∮ er1 ≡ er2 ->
-      ∮ BOP el1 op er1 : t @ i1 ≡ BOP el2 op er2 : t @ i2
-  | equive_tuple es1 es2 i1 i2 :
-      Forall2 equive es1 es2 ->
-      ∮ tup es1 @ i1 ≡ tup es2 @ i2
-  | equive_struct fs1 fs2 i1 i2 :
-      F.relfs equive fs1 fs2 ->
-      ∮ struct { fs1 } @ i1 ≡ struct { fs2 } @ i2
-  | equive_header fs1 fs2 e1 e2 i1 i2 :
-      F.relfs equive fs1 fs2 ->
-      ∮ e1 ≡ e2 ->
-      ∮ hdr { fs1 } valid:=e1 @ i1 ≡ hdr { fs2 } valid:=e2 @ i2
-  | equive_member t x e1 e2 i1 i2 :
-      ∮ e1 ≡ e2 ->
-      ∮ Mem e1 dot x : t @ i1 ≡ Mem e2 dot x : t @ i2
-  | equive_error err i1 i2 :
-      ∮ Error err @ i1 ≡ Error err @ i2
-  | equive_header_stack ts hs1 hs2 ni i1 i2 :
-      Forall2 equive hs1 hs2 ->
-      ∮ Stack hs1:ts nextIndex:=ni @ i1 ≡ Stack hs2:ts nextIndex:=ni @ i2
-  | equive_stack_access ts e1 e2 n i1 i2 :
-      ∮ e1 ≡ e2 ->
-      ∮ Access e1[n] : ts @ i1 ≡ Access e2[n] : ts @ i2
-  where "∮ e1 ≡ e2" := (equive e1 e2).
-  
-  (** Induction principle. *)
-  Section ExprEquivalenceInduction.
-    Variable tags_t : Type.
-    
-    Variable P : e tags_t -> e tags_t -> Prop.
-    
-    Hypothesis HBool : forall b i i', P <{ BOOL b @ i }> <{ BOOL b @ i' }>.
-    
-    Hypothesis HBit : forall w n i i', P <{ w W n @ i }> <{ w W n @ i' }>.
-    
-    Hypothesis HInt : forall w z i i', P <{ w S z @ i }> <{ w S z @ i' }>.
-    
-    Hypothesis HVar : forall x τ i1 i2,
-        P <{ Var x:τ @ i1 }> <{ Var x:τ @ i2 }>.
-    
-    Hypothesis HSlice : forall e1 e2 h l i1 i2,
-        ∮ e1 ≡ e2 ->
-        P e1 e2 ->
-        P <{ Slice e1 [h:l] @ i1 }> <{ Slice e2 [h:l] @ i2 }>.
-    
-    Hypothesis HCast : forall τ e1 e2 i1 i2,
-        ∮ e1 ≡ e2 ->
-        P e1 e2 ->
-        P <{ Cast e1:τ @ i1 }> <{ Cast e2:τ @ i2 }>.
-    
-    Hypothesis HUop : forall t op e1 e2 i1 i2,
-        ∮ e1 ≡ e2 ->
-        P e1 e2 ->
-        P <{ UOP op e1 : t @ i1 }> <{ UOP op e2 : t @ i2 }>.
-    
-    Hypothesis HBop : forall t op el1 er1 el2 er2 i1 i2,
-        ∮ el1 ≡ el2 ->
-        P el1 el2 ->
-        ∮ er1 ≡ er2 ->
-        P er1 er2 ->
-        P <{ BOP el1 op er1 : t @ i1 }> <{ BOP el2 op er2 : t @ i2 }>.
-    
-    Hypothesis HTup : forall es1 es2 i1 i2,
-        Forall2 equive es1 es2 ->
-        Forall2 P es1 es2 ->
-        P <{ tup es1 @ i1 }> <{ tup es2 @ i2 }>.
-    
-    Hypothesis HStruct : forall  fs1 fs2 i1 i2,
-        F.relfs equive fs1 fs2 ->
-        F.relfs P fs1 fs2 ->
-        P <{ struct { fs1 } @ i1 }> <{ struct { fs2 } @ i2 }>.
-    
-    Hypothesis HHeader : forall  fs1 fs2 e1 e2 i1 i2,
-        F.relfs equive fs1 fs2 ->
-        F.relfs P fs1 fs2 ->
-        ∮ e1 ≡ e2 ->
-        P e1 e2 ->
-        P <{ hdr { fs1 } valid:=e1 @ i1 }> <{ hdr { fs2 } valid:=e2 @ i2 }>.
-    
-    Hypothesis HMember : forall t x e1 e2 i1 i2,
-        ∮ e1 ≡ e2 ->
-        P e1 e2 ->
-        P <{ Mem e1 dot x : t @ i1 }> <{ Mem e2 dot x : t @ i2 }>.
-    
-    Hypothesis HError : forall err i1 i2,
-        P <{ Error err @ i1 }> <{ Error err @ i2 }>.
-    
-    Hypothesis HHeaderStack : forall ts hs1 hs2 ni i1 i2,
-        Forall2 equive hs1 hs2 ->
-        Forall2 P hs1 hs2 ->
-        P <{ Stack hs1:ts nextIndex:=ni @ i1 }>
-        <{ Stack hs2:ts nextIndex:=ni @ i2 }>.
-    
-    Hypothesis HAccess : forall ts e1 e2 n i1 i2,
-        ∮ e1 ≡ e2 ->
-        P e1 e2 ->
-        P <{ Access e1[n] : ts @ i1 }> <{ Access e2[n] : ts @ i2 }>.
-    
-    (** Custom induction principle. *)
-    Definition custom_equive_ind :
-      forall (e1 e2 : e tags_t), ∮ e1 ≡ e2 -> P e1 e2 :=
-      fix eeind e1 e2 (H : ∮ e1 ≡ e2) : P e1 e2 :=
-        let fix lind {es1 es2 : list (e tags_t)}
-                (Hes : Forall2 equive es1 es2) : Forall2 P es1 es2 :=
-            match Hes with
-            | Forall2_nil _ => Forall2_nil _
-            | Forall2_cons _ _ Hh Ht
-              => Forall2_cons _ _ (eeind _ _ Hh) (lind Ht)
-            end in
-        let fix fsind {fs1 fs2 : F.fs String.string (e tags_t)}
-                (Hfs : F.relfs equive fs1 fs2)
-            : F.relfs P fs1 fs2 :=
-            match Hfs with
-            | Forall2_nil _ => Forall2_nil _
-            | Forall2_cons _ _ (conj Hx He) Ht
-              => Forall2_cons _ _
-                             (conj Hx (eeind _ _ He)) (fsind Ht)
-            end in
-        match H with
-        | equive_bool b i i' => HBool b i i'
-        | equive_bit w n i i' => HBit w n i i'
-        | equive_int w z i i' => HInt w z i i'
-        | equive_var x τ i1 i2 => HVar x τ i1 i2
-        | equive_slice _ _ h l i1 i2 He
-          => HSlice _ _ h l i1 i2 He (eeind _ _ He)
-        | equive_cast τ _ _ i1 i2 He
-          => HCast τ _ _ i1 i2 He (eeind _ _ He)
-        | equive_uop t op _ _ i1 i2 He
-          => HUop t op _ _ i1 i2 He (eeind _ _ He)
-        | equive_bop t op _ _ _ _ i1 i2 Hel Her
-          => HBop
-              t op _ _ _ _ i1 i2
-              Hel (eeind _ _ Hel)
-              Her (eeind _ _ Her)
-        | equive_tuple _ _ i1 i2 Hes
-          => HTup _ _ i1 i2 Hes (lind Hes)
-        | equive_struct _ _ i1 i2 Hfs
-          => HStruct _ _ i1 i2 Hfs (fsind Hfs)
-        | equive_header _ _ _ _ i1 i2 Hfs He
-          => HHeader _ _ _ _ i1 i2 Hfs (fsind Hfs) He (eeind _ _ He)
-        | equive_member t x _ _ i1 i2 He
-          => HMember t x _ _ i1 i2 He (eeind _ _ He)
-        | equive_error err i1 i2 => HError err i1 i2
-        | equive_header_stack ts _ _ ni i1 i2 Hhs
-          => HHeaderStack ts _ _ ni i1 i2 Hhs (lind Hhs)
-        | equive_stack_access ts _ _ n i1 i2 He
-          => HAccess ts _ _ n i1 i2 He (eeind _ _ He)
-        end.
-    (**[]*)
-  End ExprEquivalenceInduction.
-  
-  Section ExprEquivalenceDefs.
-    Context {tags_t : Type}.
-    
-    Lemma equive_reflexive : Reflexive (@equive tags_t).
-    Proof.
-      unfold Reflexive; intros e;
-        induction e using custom_e_ind;
-        econstructor; eauto 2; try reflexivity;
-          try (ind_list_Forall; eauto 3; assumption);
-          try (ind_list_predfs; constructor;
-               repeat split; unravel in *; intuition).
-    Qed.
-    
-    Lemma equive_symmetric : Symmetric (@equive tags_t).
-    Proof.
-      intros ? ? ?;
-             match goal with
-             | H: ∮ _ ≡ _ |- _ => induction H using custom_equive_ind
-             end;
-        econstructor; eauto 1; try (symmetry; assumption);
-          try match goal with
-              | H: Forall2 equive ?es1 ?es2,
-                   IH: Forall2 _ ?es1 ?es2
-                |- Forall2 equive ?es2 ?es1
-                => induction H; inv IH; constructor; intuition
-              end;
-          try match goal with
-              | H: F.relfs equive ?fs1 ?fs2,
-                   IH: F.relfs _ ?fs1 ?fs2 |- F.relfs _ ?fs2 ?fs1
-                => induction H; inv IH;
-                    constructor; repeat relf_destruct;
-                      unfold equiv in *; subst;
-                        repeat split; intuition
-              end.
-    Qed.
-    
-    Lemma equive_transitive : Transitive (@equive tags_t).
-    Proof.
-      intros e1; induction e1 using custom_e_ind;
-        intros ? ? H12 H23; inv H12; inv H23;
-          econstructor; try (etransitivity; eassumption); eauto 2;
-            try match goal with
-                | H: Forall _ ?l1,
-                     H12: Forall2 equive ?l1 ?l2,
-                          H23: Forall2 equive ?l2 ?l3
-                  |- Forall2 equive ?l1 ?l3
-                  => generalize dependent l3;
-                      generalize dependent l2; induction H;
-                        intros [| ? ?] ? [| ? ?] ?;
-                               repeat match goal with
-                                      | H: Forall2 _ _ (_ :: _) |- _ => inv H
-                                      | H: Forall2 _ (_ :: _) _ |- _ => inv H
-                                      end; constructor; eauto
-                end;
-            try match goal with
-                | H: F.predfs_data _ ?f1,
-                     H12: F.relfs _ ?f1 ?f2,
-                          H23: F.relfs _ ?f2 ?f3 |- _
-                  => generalize dependent f3;
-                      generalize dependent f2; induction H;
-                        intros [| [? ?] ?] ? [| [? ?] ?] ?;
-                               try match goal with
-                                   | H: F.predf_data _ ?x |- _ => destruct x as [? [? ?]]
-                                   end;
-                        repeat match goal with
-                               | H: F.relfs _ _ (_ :: _) |- _ => inv H
-                               | H: F.relfs _ (_ :: _) _ |- _ => inv H
-                               end; constructor;
-                          repeat relf_destruct; unravel in *; intuition;
-                            repeat split; unravel; intuition; eauto 2;
-                              try match goal with
-                                  | IH: forall _, _ -> forall _, _ -> _ |- _ => eapply IH; eauto 1
-                                  end; etransitivity; eauto 1
-                end.
-    Qed.
-    
-    (** Decidable Expression Equivalence. *)
-    Fixpoint eqbe (e1 e2 : e tags_t) : bool :=
-      let fix lstruct (es1 es2 : list (e tags_t)) : bool :=
-          match es1, es2 with
-          | [], _::_ | _::_, [] => false
-          | [], [] => true
-          | e1::es1, e2::es2 => eqbe e1 e2 && lstruct es1 es2
-          end in
-      let fix efsstruct (fs1 fs2 : F.fs String.string (e tags_t)) : bool :=
-          match fs1, fs2 with
-          | [], _::_ | _::_, [] => false
-          | [], [] => true
-          | (x1, e1)::fs1, (x2, e2)::fs2
-            => equiv_dec x1 x2 &&&& eqbe e1 e2 && efsstruct fs1 fs2
-          end in
-      match e1, e2 with
-      | <{ BOOL b1 @ _ }>, <{ BOOL b2 @ _ }> => eqb b1 b2
-      | <{ w1 W n1 @ _ }>, <{ w2 W n2 @ _ }>
-        => (w1 =? w2)%N && (n1 =? n2)%Z
-      | <{ w1 S z1 @ _ }>, <{ w2 S z2 @ _ }>
-        => (w1 =? w2)%positive && (z1 =? z2)%Z
-      | <{ Var x1:τ1 @ _ }>, <{ Var x2:τ2 @ _ }>
-        => equiv_dec x1 x2 &&&& eqbt τ1 τ2
-      | <{ Slice e1 [h1:l1] @ _ }>, <{ Slice e2 [h2:l2] @ _ }>
-        => (h1 =? h2)%positive && (l1 =? l2)%positive && eqbe e1 e2
-      | <{ Cast e1:τ1 @ _ }>, <{ Cast e2:τ2 @ _ }>
-        => eqbt τ1 τ2 && eqbe e1 e2
-      | <{ UOP u1 e1 : t1 @ _ }>, <{ UOP u2 e2 : t2 @ _ }>
-        => equiv_dec u1 u2 &&&& eqbe e1 e2 && eqbt t1 t2
-      | <{ BOP el1 o1 er1 : t1 @ _ }>,
-        <{ BOP el2 o2 er2 : t2 @ _ }>
-        => equiv_dec o1 o2 &&&& eqbe el1 el2 && eqbe er1 er2 && eqbt t1 t2
-      | <{ tup es1 @ _ }>, <{ tup es2 @ _ }> => lstruct es1 es2
-      | <{ struct { fs1 } @ _ }>, <{ struct { fs2 } @ _ }>
-        => efsstruct fs1 fs2
-      | <{ hdr { fs1 } valid:=e1 @ _ }>,
-        <{ hdr { fs2 } valid:=e2 @ _ }>
-        => eqbe e1 e2 && efsstruct fs1 fs2
-      | <{ Mem e1 dot x1 : t1 @ _ }>, <{ Mem e2 dot x2 : t2 @ _ }>
-        => equiv_dec x1 x2 &&&& eqbe e1 e2 && eqbt t1 t2
-      | <{ Error err1 @ _ }>, <{ Error err2 @ _ }>
-        => if equiv_dec err1 err2 then true else false
-      | <{ Stack hs1:ts1 nextIndex:=ni1 @ _ }>,
-        <{ Stack hs2:ts2 nextIndex:=ni2 @ _ }>
-        => (ni1 =? ni2)%Z && F.eqb_fs eqbt ts1 ts2 && lstruct hs1 hs2
-      | <{ Access hs1[n1] : ts1 @ _ }>,
-        <{ Access hs2[n2] : ts2 @ _ }>
-        => eqb_list ts1 ts2 &&&& (n1 =? n2)%Z && eqbe hs1 hs2
-      | _, _ => false
-      end.
-    (**[]*)
-    
-    Import F.RelfEquiv.
-    
-    Hint Rewrite eqb_reflx.
-    Hint Rewrite Pos.eqb_refl.
-    Hint Rewrite Z.eqb_refl.
-    Hint Rewrite eqbt_refl.
-    Hint Rewrite equiv_dec_refl.
-    Local Hint Extern 5 => equiv_dec_refl_tactic : core.
-    Hint Rewrite (@relop_eq String.string).
-    Hint Rewrite @eqb_list_refl.
-    
-    (* TODO: somehow using a hidden axiom as an assumption. *)
-    Lemma equive_eqbe : forall e1 e2 : e tags_t,
-        ∮ e1 ≡ e2 -> eqbe e1 e2 = true.
-    Proof.
-      intros ? ? ?;
-             match goal with
-             | H: ∮ _ ≡ _ |- _ => induction H using custom_equive_ind
-             end; unravel in *; autorewrite with core; auto 1;
-        repeat match goal with
-               | H: ?trm = true |- context [ ?trm ] => rewrite H; clear H
-               end; auto 1;
-          try match goal with
-              | H: Forall2 equive ?es1 ?es2,
-                   IH: Forall2 _ ?es1 ?es2 |- _
-                => induction H; inv IH; unravel in *; auto 1; intuition
-              end;
-          try match goal with
-              | H: F.relfs _ ?fs1 ?fs2,
-                   IH: F.relfs _ ?fs1 ?fs2 |- _
-                => induction H; inv IH; auto 1;
-                    match goal with
-                    | H: F.relf _ ?f1 ?f2 |- _
-                      => destruct f1 as [? ?];
-                          destruct f2 as [? ?];
-                          repeat relf_destruct; unravel in *;
-                            unfold equiv in *;
-                            intuition; subst;
-                              autorewrite with core;
-                              try equiv_dec_refl_tactic
-                    end
-              end;
-          repeat match goal with
-                 | H: ?trm = true |- context [ ?trm ] => rewrite H; clear H
-                 end; auto 1;
-            try match goal with
-                | |- context [ F.eqb_fs eqbt ?ts ?ts ]
-                  => rewrite (equiv_eqb_fs _ _ eqbt_reflect ts ts);
-                      unfold equiv in *; auto 1; try reflexivity
-                end;
-            try (equiv_dec_refl_tactic; auto 1;
-                 autorewrite with core in *; contradiction).
-      rewrite N.eqb_refl; tauto.
-    Qed.
-    
-    Ltac eq_true_terms :=
-      match goal with
-      | H: eqb _ _ = true |- _
-        => apply eqb_prop in H; subst
-      | H: (_ =? _)%N = true |- _
-        => apply InitialRing.Neqb_ok in H; subst
-      | H: (_ =? _)%positive = true |- _
-        => apply Peqb_true_eq in H; subst
-      | H: (_ =? _)%Z = true |- _
-        => apply Z.eqb_eq in H; subst
-      | H: _ && _ = true |- _
-        => apply andb_true_iff in H as [? ?]
-      | H: context [equiv_dec ?x1 ?x2 &&&& _] |- _
-        => destruct (equiv_dec x1 x2) as [? | ?];
-          unravel in H; try discriminate
-      | H: context [if equiv_dec ?t1 ?t2 then _ else _] |- _
-        => destruct (equiv_dec t1 t2) as [? | ?];
-          unravel in H; try discriminate
-      | H: context [if eqbt ?t1 ?t2 then _ else _] |- _
-        => destruct (eqbt t1 t2) eqn:?;
-                   unravel in H; try discriminate
-      | H: context [eqbt ?t1 ?t2 && _] |- _
-        => destruct (eqbt t1 t2) eqn:?;
-                   unravel in H; try discriminate
-      | H: context [eqbe ?e1 ?e2 && _] |- _
-        => destruct (eqbe e1 e2) eqn:?;
-                   unravel in H; try discriminate
-      | H: eqbt _ _ = true |- _
-        => apply eqbt_eq_iff in H
-      | H: context [if eqbe ?e1 ?e2 then _ else _] |- _
-        => destruct (eqbe e1 e2) eqn:?;
-                   unravel in H; try discriminate
-      | H: eqbe ?e1 _ = true,
-           IH: forall e2, eqbe ?e1 e2 = true -> ∮ ?e1 ≡ e2 |- _
-        => apply IH in H
-      | H: _ === _ |- _ => unfold equiv in H;
+  Ltac eq_true_terms :=
+    match goal with
+    | H: eqb _ _ = true |- _
+      => apply eqb_prop in H; subst
+    | H: (_ =? _)%N = true |- _
+      => apply InitialRing.Neqb_ok in H; subst
+    | H: (_ =? _)%positive = true |- _
+      => apply Peqb_true_eq in H; subst
+    | H: (_ =? _)%Z = true |- _
+      => apply Z.eqb_eq in H; subst
+    | H: _ && _ = true |- _
+      => apply andb_true_iff in H as [? ?]
+    | H: context [equiv_dec ?x1 ?x2 &&&& _] |- _
+      => destruct (equiv_dec x1 x2) as [? | ?];
+        unravel in H; try discriminate
+    | H: context [if equiv_dec ?t1 ?t2 then _ else _] |- _
+      => destruct (equiv_dec t1 t2) as [? | ?];
+        unravel in H; try discriminate
+    | H: context [if eqbt ?t1 ?t2 then _ else _] |- _
+      => destruct (eqbt t1 t2) eqn:?;
+                 unravel in H; try discriminate
+    | H: context [eqbt ?t1 ?t2 && _] |- _
+      => destruct (eqbt t1 t2) eqn:?;
+                 unravel in H; try discriminate
+    | H: context [eqbe ?e1 ?e2 && _] |- _
+      => destruct (eqbe e1 e2) eqn:?;
+                 unravel in H; try discriminate
+    | H: eqbt _ _ = true |- _
+      => apply eqbt_eq_iff in H
+    | H: context [if eqbe ?e1 ?e2 then _ else _] |- _
+      => destruct (eqbe e1 e2) eqn:?;
+                 unravel in H; try discriminate
+    | H: eqbe ?e1 _ = true,
+        IH: forall e2, eqbe ?e1 e2 = true -> ?e1 = e2 |- _
+      => apply IH in H
+    | H: _ === _ |- _ => unfold equiv in H;
+                       match goal with
+                       | H: _ = _ |- _ => subst
+                       end
+    | H: equiv _ _ |- _ => unfold equiv in H;
                          match goal with
                          | H: _ = _ |- _ => subst
                          end
-      | H: equiv _ _ |- _ => unfold equiv in H;
-                           match goal with
-                           | H: _ = _ |- _ => subst
-                           end
-      | H: Forall _ (_ :: _) |- _ => inv H
-      | H: ?P, IH: ?P -> ?Q |- _ => apply IH in H as ?
-      | H: (if ?trm then true else false) = true |- _
-        => destruct trm eqn:?; unravel in H; try discriminate
-      | H: relop _ _ _ |- _ => inv H
-      | H: F.eqb_fs eqbt _ _ = true
-        |- _ => pose proof eqb_fs_equiv _ _ eqbt_reflect _ _ H as ?; clear H
-      | H: F.relfs eq _ _ |- _ => apply eq_relfs in H; subst
-      end.
-    (**[]*)
+    | H: Forall _ (_ :: _) |- _ => inv H
+    | H: ?P, IH: ?P -> ?Q |- _ => apply IH in H as ?
+    | H: (if ?trm then true else false) = true |- _
+      => destruct trm eqn:?; unravel in H; try discriminate
+    end.
     
-    Local Hint Constructors equive : core.
-    Local Hint Extern 5 => eq_true_terms : core.
+  Local Hint Extern 5 => eq_true_terms : core.
     
-    Lemma eqbe_equive : forall e1 e2 : e tags_t,
-        eqbe e1 e2 = true -> equive e1 e2.
-    Proof.
-      induction e1 using custom_e_ind;
-        intros [] ?; unravel in *;
-        try discriminate; auto 1;
-          repeat eq_true_terms;
-          unfold equiv in *;
-          subst; auto; try constructor; auto 1;
-            try match goal with
-                | |- Forall2 _ ?es1 ?es2
-                  => generalize dependent es2;
-                      induction es1; intros [];
-                        unravel in *; try discriminate; auto 5
-                end;
-            try match goal with
-                | |- F.relfs _ ?fs1 ?fs2
-                  => generalize dependent fs2;
-                      induction fs1 as [| [? ?] ? ?];
-                      intros [| [? ?] ?]; intros;
-                        unravel in *; try discriminate; auto 1;
-                          try destruct_lifted_andb; repeat destruct_andb;
-                            try invert_cons_predfs; repeat constructor;
-                              intuition; unfold F.relfs in *; auto 2
-                end.
-      destruct (eqb_list rt result_hdr_type) eqn:Hb;
-        try discriminate.
-      repeat eq_true_terms.
-      rewrite eqb_list_iff in Hb; subst; auto.
-    Qed.
-    
-    Local Hint Resolve equive_eqbe : core.
-    Local Hint Resolve eqbe_equive : core.
-    
-    Lemma equive_eqbe_iff : forall e1 e2 : e tags_t,
-        ∮ e1 ≡ e2 <-> eqbe e1 e2 = true.
-    Proof. intros; split; auto 2. Qed.
-    
-    Hint Resolve equive_eqbe_iff : core.
-    Hint Extern 5 =>
-    match goal with
-    | H: eqbe ?e1 ?e2 = false,
-         H': ∮ ?e1 ≡ ?e2 |- False
-      => apply equive_eqbe_iff in H';
-  rewrite H' in H; discriminate
-    end : core.
-    
-    Lemma equive_reflect : forall e1 e2 : e tags_t,
-        reflect (∮ e1 ≡ e2) (eqbe e1 e2).
-    Proof.
-      intros; reflect_split; auto 2;
-        autorewrite with core; auto 2.
-    Qed.
-  End ExprEquivalenceDefs.
+  Lemma eqbe_eq : forall e1 e2 : e,
+      (e1 =? e2)%expr = true -> e1 = e2.
+  Proof.
+    induction e1 using custom_e_ind;
+      intros [] ?; unravel in *;
+      try discriminate; auto 1;
+      repeat eq_true_terms;
+      unfold equiv in *;
+      subst; auto; try constructor; auto 1; f_equal; auto.
+    - rename fields into l1; rename fields0 into l2.
+      generalize dependent l2.
+      clear dependent valid; clear valid0.
+      ind_list_Forall; intros [| h2 l2] He; try discriminate; auto.
+      apply andb_prop in He as [He1 He2]; f_equal; eauto.
+    - inv H0; destruct valid0; cbn in *; try discriminate; f_equal; auto.
+    - rewrite relop_eq in e0; assumption.
+  Qed.
   
-  Local Hint Resolve equive_reflexive : core.
-  Local Hint Resolve equive_symmetric : core.
-  Local Hint Resolve equive_transitive : core.
+  Local Hint Resolve eqbe_refl : core.
+  Local Hint Resolve eqbe_eq : core.
+    
+  Lemma eqbe_iff : forall e1 e2 : e,
+      (e1 =? e2)%expr = true <-> e1 = e2.
+  Proof. intros; split; intros; subst; auto. Qed.
+    
+  Hint Resolve eqbe_iff : core.
+  Hint Extern 5 =>
+         match goal with
+         | H: eqbe ?e1 ?e2 = false,
+             H': ?e1 = ?e2 |- False
+           => apply eqbe_iff in H'; rewrite H' in H; discriminate
+  end : core.
   
-  Global Instance ExprEquiv {tags_t : Type} : Equivalence (@equive tags_t).
-  Proof. constructor; auto 1. Defined.
+  Lemma eqbe_reflect : forall e1 e2 : e,
+      reflect (e1 = e2) (e1 =? e2)%expr.
+  Proof.
+    intros; reflect_split; auto 2;
+      autorewrite with core; auto 2.
+  Qed.
+End ExprEquivalenceDefs.
   
-  Global Instance ExprEqDec {tags_t : Type} : EqDec (e tags_t) equive :=
-    { equiv_dec := fun e1 e2 => reflect_dec _ _ (equive_reflect e1 e2) }.
-  (**[]*)
-End ExprEquivalence.
+Global Instance ExprEqDec {tags_t : Type} : EqDec e eq :=
+  { equiv_dec := fun e1 e2 => reflect_dec _ _ (eqbe_reflect e1 e2) }.
