deps/poulet4/lib/P4cub/Syntax/IndPrincip.v
@@ -1,241 +1,183 @@
-Set Warnings "custom-entry-overridden,parsing".
 Require Import Coq.PArith.BinPosDef Coq.PArith.BinPos
         Coq.ZArith.BinIntDef Coq.ZArith.BinInt.
 Require Import Poulet4.P4cub.Syntax.AST
         Poulet4.P4cub.Syntax.CubNotations.
-Import String.
+Import String Expr ExprNotations.
 
 (** Custom induction principle for [t]. *)
 Section TypeInduction.
-  Import Expr TypeNotations.
+  Local Open Scope ty_scope.
   
   (** An arbitrary property. *)
   Variable P : t -> Prop.
 
-  Hypothesis HTVar : forall X : string, P {{ X }}.
+  Hypothesis HTVar : forall X : nat, P X.
   
-  Hypothesis HTBool : P {{ Bool }}.
+  Hypothesis HTBool : P TBool.
   
-  Hypothesis HTBit : forall w, P {{ bit<w> }}.
+  Hypothesis HTBit : forall w, P (TBit w).
   
-  Hypothesis HTInt : forall w, P {{ int<w> }}.
+  Hypothesis HTInt : forall w, P (TInt w).
   
-  Hypothesis HTError : P {{ error }}.
+  Hypothesis HTError : P TError.
   
-  Hypothesis HTTuple : forall ts,
-      Forall P ts -> P {{ tuple ts }}.
-  
-  Hypothesis HTStruct : forall fields,
-      F.predfs_data P fields -> P {{ struct { fields } }}.
-  
-  Hypothesis HTHeader : forall fields,
-      F.predfs_data P fields -> P {{ hdr { fields } }}.
-  
-  Hypothesis HTHeaderStack : forall fields size,
-      F.predfs_data P fields -> P {{ stack fields[size] }}.
-  
+  Hypothesis HTStruct : forall ts b,
+      Forall P ts -> P (TStruct ts b).
+
   (** A custom induction principle.
       Do [induction ?t using custom_t_ind]. *)
   Definition custom_t_ind : forall ty : t, P ty :=
     fix custom_t_ind (type : t) : P type :=
-      let fix list_ind (ts : list t) :
+      let fix list_ind ts :
             Forall P ts :=
-          match ts with
-          | [] => Forall_nil _
-          | h :: ts => Forall_cons _ (custom_t_ind h) (list_ind ts)
-          end in
-      let fix fields_ind
-              (flds : F.fs string t) : F.predfs_data P flds :=
-          match flds with
-          | [] => Forall_nil (F.predf_data P)
-          | (_, hft) as hf :: tf
-            => Forall_cons hf (custom_t_ind hft) (fields_ind tf)
-          end in
+        match ts with
+        | []     => Forall_nil _
+        | h :: ts => Forall_cons _ (custom_t_ind h) (list_ind ts)
+        end in
       match type with
-      | TVar X => HTVar X
-      | {{ Bool }} => HTBool
-      | {{ bit<w> }} => HTBit w
-      | {{ int<w> }} => HTInt w
-      | {{ error }} => HTError
-      | {{ tuple ts }}  => HTTuple ts (list_ind ts)
-      | {{ struct { fields } }} => HTStruct fields (fields_ind fields)
-      | {{ hdr { fields } }} => HTHeader fields (fields_ind fields)
-      | {{ stack fields[n] }} => HTHeaderStack fields n (fields_ind fields)
+      | TVar X       => HTVar X
+      | TBool        => HTBool
+      | TBit w       => HTBit w
+      | TInt w       => HTInt w
+      | TError       => HTError
+      | TStruct ts b => HTStruct ts b (list_ind ts)
       end.
   (**[]*)
 End TypeInduction.
 
 (** A custom induction principle for [e]. *)
 Section ExprInduction.
-  Import Expr.
-  Import TypeNotations.
-  Import UopNotations.
-  Import ExprNotations.
-  Import BopNotations.
+  Local Open Scope expr_scope.
   
   (** An arbitrary predicate. *)
-  Variable tags_t : Type.
+  Variable P : e -> Prop.
   
-  Variable P : e tags_t -> Prop.
+  Hypothesis HEBool : forall b : bool, P b.
   
-  Hypothesis HEBool : forall b i, P <{ BOOL b @ i }>.
+  Hypothesis HEBit : forall w n, P (w `W n).
   
-  Hypothesis HEBit : forall w n i, P <{ w W n @ i }>.
+  Hypothesis HEInt : forall w n, P (w `S n).
   
-  Hypothesis HEInt : forall w n i, P <{ w S n @ i }>.
+  Hypothesis HEVar : forall ty x, P (EVar ty x).
   
-  Hypothesis HEVar : forall (ty : t) (x : string) i,
-      P <{ Var x : ty @ i }>.
+  Hypothesis HESlice : forall n hi lo, P n -> P (ESlice n hi lo).
   
-  Hypothesis HESlice : forall n hi lo i,
-      P n -> P <{ Slice n [ hi : lo ] @ i }>.
+  Hypothesis HECast : forall τ exp, P exp -> P (ECast τ exp).
   
-  Hypothesis HECast : forall τ exp i,
-      P exp -> P <{ Cast exp:τ @ i }>.
+  Hypothesis HEUop : forall rt op exp, P exp -> P (EUop rt op exp).
   
-  Hypothesis HEUop : forall (rt : t) (op : uop) (ex : e tags_t) i,
-      P ex -> P <{ UOP op ex : rt @ i }>.
+  Hypothesis HEBop : forall rt op lhs rhs,
+      P lhs -> P rhs -> P (EBop rt op lhs rhs).
   
-  Hypothesis HEBop : forall rt (op : bop) (lhs rhs : e tags_t) i,
-      P lhs -> P rhs -> P <{ BOP lhs op rhs : rt @ i }>.
+  Hypothesis HEStruct : forall fields valid,
+      Forall P fields -> predop P valid -> P (EStruct fields valid).
   
-  Hypothesis HETuple : forall es i,
-      Forall P es -> P <{ tup es @ i }>.
+  Hypothesis HEExprMember : forall rt x exp,
+      P exp -> P (EMember rt x exp).
   
-  Hypothesis HEStruct : forall fields i,
-      F.predfs_data P fields -> P <{ struct {fields} @ i }>.
-  
-  Hypothesis HEHeader : forall fields b i,
-      P b -> F.predfs_data P fields ->
-      P <{ hdr {fields} valid:=b @ i }>.
-  
-  Hypothesis HEExprMember : forall rt x expr i,
-      P expr -> P <{ Mem expr dot x : rt @ i }>.
-  
-  Hypothesis HEError : forall err i, P <{ Error err @ i }>.
-  
-  Hypothesis HEStack : forall ts hs ni i,
-      Forall P hs ->
-      P <{ Stack hs:ts nextIndex:=ni @ i }>.
-  
-  Hypothesis HAccess : forall rt e n i,
-      P e -> P <{ Access e[n] : rt @ i }>.
-  
+  Hypothesis HEError : forall err, P (EError err).
+    
   (** A custom induction principle.
       Do [induction ?e using custom_e_ind]. *)
-  Definition custom_e_ind : forall exp : e tags_t, P exp :=
-    fix eind (expr : e tags_t) : P expr :=
-      let fix fields_ind (flds : F.fs string (e tags_t))
-          : F.predfs_data P flds :=
-          match flds with
-          | [] => Forall_nil _
-          | (_, hfe) as hf :: tf
-            => Forall_cons hf (eind hfe) (fields_ind tf)
-          end in
-      let fix list_ind (es : list (e tags_t)) : Forall P es :=
+  Definition custom_e_ind : forall exp : e, P exp :=
+    fix eind (expr : e) : P expr :=
+      let fix list_ind (es : list e) : Forall P es :=
           match es with
-          | [] => Forall_nil P
+          | []        => Forall_nil P
           | exp :: ees => Forall_cons exp (eind exp) (list_ind ees)
           end in
+      let opind (o : option e) : predop P o :=
+        match o with
+        | Some exp => predop_some _ _ (eind exp)
+        | None     => predop_none _
+        end in
       match expr with
-      | <{ BOOL b @ i }> => HEBool b i
-      | <{ w W n @ i }>  => HEBit w n i
-      | <{ w S n @ i }>  => HEInt w n i
-      | <{ Var x:ty @ i }> => HEVar ty x i
-      | <{ Slice n [h:l] @ i }> => HESlice n h l i (eind n)
-      | <{ Cast exp:τ @ i }> => HECast τ exp i (eind exp)
-      | <{ UOP op exp : t @ i }> => HEUop t op exp i (eind exp)
-      | <{ BOP lhs op rhs : t @ i }>
-        => HEBop t op lhs rhs i (eind lhs) (eind rhs)
-      | <{ tup es @ i }>         => HETuple es i (list_ind es)
-      | <{ struct { fields } @ i }> => HEStruct fields i (fields_ind fields)
-      | <{ hdr { fields } valid:=b @ i }>
-        => HEHeader fields b i (eind b) (fields_ind fields)
-      | <{ Mem exp dot x : rt @ i }> => HEExprMember rt x exp i (eind exp)
-      | <{ Error err @ i }> => HEError err i
-      | <{ Stack hs:ts nextIndex:=ni @ i }>
-        => HEStack ts hs ni i (list_ind hs)
-      | <{ Access e[n] : rt @ i }> => HAccess rt e n i (eind e)
+      | EBool b       => HEBool b
+      | w `W n        => HEBit w n
+      | w `S n        => HEInt w n
+      | EVar ty x     => HEVar ty x
+      | ESlice n h l  => HESlice n h l (eind n)
+      | ECast τ exp   => HECast τ exp (eind exp)
+      | EUop τ op exp => HEUop τ op exp (eind exp)
+      | EBop τ op lhs rhs
+        => HEBop τ op lhs rhs (eind lhs) (eind rhs)
+      | EStruct fields valid
+        => HEStruct fields valid (list_ind fields) (opind valid)
+      | EMember rt x exp => HEExprMember rt x exp (eind exp)
+      | EError err       => HEError err
       end.
   (**[]*)
 End ExprInduction.
 
+Import Parser ParserNotations.
+
 (** A custom induction principle for select patterns. *)
 Section PatternInduction.
-  Import Parser.
-  Import ParserNotations.
-      
+  Local Open Scope pat_scope.
+  
   Variable P : pat -> Prop.
       
-  Hypothesis HWild : P [{ ?? }].
+  Hypothesis HWild : P PATWild.
   
   Hypothesis HMask : forall p1 p2,
-      P p1 -> P p2 -> P [{ p1 &&& p2 }].
+      P p1 -> P p2 -> P (PATMask p1 p2).
   
   Hypothesis HRange : forall p1 p2,
-      P p1 -> P p2 -> P [{ p1 .. p2 }].
+      P p1 -> P p2 -> P (PATRange p1 p2).
   
-  Hypothesis HBit : forall w n, P [{ w PW n }].
+  Hypothesis HBit : forall w n, P (w PW n).
   
-  Hypothesis HInt : forall w n, P [{ w PS n }].
+  Hypothesis HInt : forall w n, P (w PS n).
   
-  Hypothesis HTuple : forall ps,
-      Forall P ps -> P [{ PTUP ps }].
+  Hypothesis HStruct : forall ps,
+      Forall P ps -> P (PATStruct ps).
   
-  (** A custom induction principle,
+  (** A customnduction principle,
       do [induction ?H using custom_pat_ind]. *)
   Definition custom_pat_ind : forall (p : pat), P p :=
     fix pind (p : pat) : P p :=
       let fix lind (ps : list pat) : Forall P ps :=
-          match ps with
-          | [] => Forall_nil _
-          | p::ps => Forall_cons p (pind p) (lind ps)
-          end in
+        match ps with
+        | []   => Forall_nil _
+        | p::ps => Forall_cons p (pind p) (lind ps)
+        end in
       match p with
-      | [{ ?? }] => HWild
-      | [{ p1 &&& p2 }] => HMask p1 p2 (pind p1) (pind p2)
-      | [{ p1 .. p2 }] => HRange p1 p2 (pind p1) (pind p2)
-      | [{ w PW n }] => HBit w n
-      | [{ w PS z }] => HInt w z
-      | [{ PTUP ps }] => HTuple ps (lind ps)
+      | PATWild        => HWild
+      | PATMask p1 p2  => HMask p1 p2 (pind p1) (pind p2)
+      | PATRange p1 p2 => HRange p1 p2 (pind p1) (pind p2)
+      | w PW n         => HBit w n
+      | w PS z         => HInt w z
+      | PATStruct ps   => HStruct ps (lind ps)
       end.
   (**[]*)
 End PatternInduction.
 
-(** A custom induction principle for parser expressions. *)
+(** A customnduction principle for parser expressions. *)
 Section ParserExprInduction.
-  Import Parser.
-  Import ParserNotations.
-  Import ExprNotations.
-  
-  Context {tags_t : Type}.
-  
   (** An arbitrary predicate. *)
-  Variable P : e tags_t -> Prop.
+  Variable P : e -> Prop.
   
-  Hypothesis HState : forall st i, P p{ goto st @ i }p.
+  Hypothesis HState : forall st, P (PGoto st).
   
-  Hypothesis HSelect : forall exp st cases i,
-      F.predfs_data P cases ->
-      P st -> 
-      P p{ select exp { cases } default:=st @ i }p.
-  (**[]*)
+  Hypothesis HSelect : forall exp st cases,
+      Field.predfs_data P cases -> P st -> 
+      P (PSelect exp st cases).
   
-  (** A custom induction principle,
+  (** A customnduction principle,
       do [induction ?H using pe_ind] *)
-  Definition pe_ind : forall pe : e tags_t, P pe :=
+  Definition pe_ind : forall pe : e, P pe :=
     fix peind pe : P pe :=
-      let fix fsind {A : Type} (es : F.fs A (e tags_t))
-          : F.predfs_data P es :=
+      let fix fsind {A : Set} (es : Field.fs A e)
+        : Field.predfs_data P es :=
           match es with
           | [] => Forall_nil _
           | (_,pe) as epe :: es =>
             Forall_cons epe (peind pe) (fsind es)
           end in
       match pe with
-      | p{ goto st @ i }p => HState st i
-      | p{ select exp { cases } default:=st @ i }p
-        => HSelect exp st _ i (fsind cases) (peind st)
+      | PGoto st => HState st
+      | PSelect exp st cases
+        => HSelect exp st _ (fsind cases) (peind st)
       end.
   (**[]*)
 End ParserExprInduction.
